Isabelle/Norm_proofs.thy
@@ -307,20 +307,18 @@ lemma un_minimal:
 using rn_mnotr mn_rn assms(2,1,3-4) unfolding update_norms_def .
 
 
-(*****************************************************************************
-  iterate_norms2
- *****************************************************************************)
+subsection {* @{text iterate_norms} *}
 
-lemma itno2_induct [case_names Base Step]:
+lemma itno_induct [case_names Base Step]:
   assumes B: "P ([], gr)"
       and S: "\<And>norms rest yes no.
                 itno_invariant gr norms rest \<Longrightarrow>
                 partition (v_rule_has_norm norms) rest = (yes, no) \<Longrightarrow>
                 P (norms, rest) \<Longrightarrow>
                 P (update_norms gr norms yes, no)"
-  shows "P (iterate_norms2 gr)"
-    and "itno_invariant gr (fst (iterate_norms2 gr)) (snd (iterate_norms2 gr))"
-  unfolding iterate_norms2_def
+  shows "P (iterate_norms gr)"
+    and "itno_invariant gr (fst (iterate_norms gr)) (snd (iterate_norms gr))"
+  unfolding iterate_norms_def
 proof (induct rule: pi_induct)
   case Base
     case 1 show ?case using B by auto
@@ -338,7 +336,7 @@ next
       show ?case using I1 I2 unfolding itno_invariant_def by auto
 qed
 
-lemma itno2_induct_sd [case_names Base Step]:
+lemma itno_induct_sd [case_names Base Step]:
   assumes B: "P ([], gr)"
       and S: "\<And>norms rest yes no.
                 itno_invariant gr norms rest \<Longrightarrow>
@@ -347,9 +345,9 @@ lemma itno2_induct_sd [case_names Base Step]:
                 P (norms, rest) \<Longrightarrow>
                 P (update_norms gr norms yes, no)"
       and G: "gram_sd gr"
-  shows "P (iterate_norms2 gr)"
-    and "itno_invariant_sd gr (fst (iterate_norms2 gr)) (snd (iterate_norms2 gr))"
-proof (induct rule: itno2_induct(1))
+  shows "P (iterate_norms gr)"
+    and "itno_invariant_sd gr (fst (iterate_norms gr)) (snd (iterate_norms gr))"
+proof (induct rule: itno_induct(1))
   case Base
     case 1 show ?case using B by auto
     case 2 show ?case unfolding itno_invariant_sd_def using gsd_alist[OF G] by auto
@@ -384,12 +382,37 @@ next
     show ?case using Step unfolding itno_invariant_sd_def using I1 I2 I3 by auto
 qed
 
-lemma nog_invariant_holds':
+lemma itno_invariant_holds: "itno_invariant gr (fst (iterate_norms gr)) (snd (iterate_norms gr))"
+using itno_induct(2) by auto
+
+lemma itno_gr_keys_equal:
+  "keys gr = keys (fst (iterate_norms gr)) \<union> keys (snd (iterate_norms gr))"
+using itno_invariant_holds[of gr] unfolding itno_invariant_def by auto
+
+lemma itno_invariant_sd_holds:
+  assumes "gram_sd gr"
+    shows "itno_invariant_sd gr (fst (iterate_norms gr)) (snd (iterate_norms gr))"
+using itno_induct_sd(2) assms by auto
+
+
+(*****************************************************************************
+  gram_nsd_fun
+ *****************************************************************************)
+
+lemma gram_nsd_sd: "gram_nsd_fun gr \<Longrightarrow> gram_sd gr"
+by (simp add: gram_nsd_fun_def)
+
+
+(*****************************************************************************
+  norms_of_grammar
+ *****************************************************************************)
+
+lemma nog_invariant_holds:
   assumes "gram_sd gr"
       and "(v, rules) \<in> set gr"
-      and "v \<in> keys (norms_of_grammar2 gr)"
-  shows "nog_invariant_n_t_vs (norms_of_grammar2 gr) v rules"
-using assms(3) unfolding norms_of_grammar2_def proof (induct rule: itno2_induct_sd(1))
+      and "v \<in> keys (norms_of_grammar gr)"
+  shows "nog_invariant_n_t_vs (norms_of_grammar gr) v rules"
+using assms(3) unfolding norms_of_grammar_def proof (induct rule: itno_induct_sd(1))
   case (Step norms rest yes no)
   def un \<equiv> "update_norms gr norms yes"
   have P: "v \<in> keys un" unfolding un_def using Step(5) by simp
@@ -423,168 +446,23 @@ qed (auto simp add: assms(1))
 
 lemma nog_invariant_n_t_vs_holds:
   assumes "gram_sd gr"
-      and "(v, n, t, vs) \<in> set (norms_of_grammar2 gr)"
       and "(v, rules) \<in> set gr"
-    shows "nog_invariant (norms_of_grammar2 gr) rules n t vs"
+      and "(v, n, t, vs) \<in> set (norms_of_grammar gr)"
+    shows "nog_invariant (norms_of_grammar gr) rules n t vs"
 proof -
-  def norms \<equiv> "(norms_of_grammar2 gr)"
-  have "nog_invariant_n_t_vs norms v rules" using nog_invariant_holds'[OF assms(1,3)] assms(2)
-    unfolding norms_of_grammar2_def norms_def by auto
+  def norms \<equiv> "(norms_of_grammar gr)"
+  have "nog_invariant_n_t_vs norms v rules" using nog_invariant_holds[OF assms(1,2)] assms(3)
+    unfolding norms_of_grammar_def norms_def by auto
   then have I: "t_rules_have_norm norms rules" "(v, min_norm_of_t_rules norms rules) \<in> set norms"
     unfolding nog_invariant_n_t_vs_def by auto
 
-  have AN: "is_alist norms" sorry
+  have II: "is_alist norms" using itno_invariant_sd_holds[OF assms(1)]
+    unfolding itno_invariant_sd_def norms_def norms_of_grammar_def by auto
   have I2: "(n, t, vs) = min_norm_of_t_rules norms rules"
-    using alist_values_equal AN assms(2) I(2) unfolding norms_def .
+    using alist_values_equal II assms(3) I(2) unfolding norms_def .
 
   show ?thesis using I(1) I2 unfolding nog_invariant_def norms_def by auto
 qed
-
-
-(*****************************************************************************
-  iterate_norms
- *****************************************************************************)
-
-lemma itno_induct [case_names Base Step]:
-  assumes B: "P ([], gr)"
-      and S: "\<And>norms rest yes no.
-                itno_invariant gr norms rest \<Longrightarrow>
-                partition (v_rule_has_norm norms) rest = (yes, no) \<Longrightarrow>
-                P (norms, rest) \<Longrightarrow>
-                P (add_norms norms yes, no)"
-  shows "P (iterate_norms gr)"
-    and "itno_invariant gr (fst (iterate_norms gr)) (snd (iterate_norms gr))"
-  unfolding iterate_norms_def
-proof (induct rule: pi_induct)
-  case Base
-    case 1 show ?case using B by auto
-    case 2 show ?case unfolding itno_invariant_def by auto
-next
-  case (Step norms rest yes no)
-    case 1 show ?case using S Step by auto
-    case 2
-      have I1: "set no \<subseteq> set gr" using Step(2-3) unfolding itno_invariant_def by auto
-      
-      have "keys gr = keys norms \<union> keys rest" using Step(2) unfolding itno_invariant_def by simp
-      then have I2: "keys gr = keys (add_norms norms yes) \<union> keys no"
-        unfolding an_keys[of norms yes] using Step(3) by force
-
-      show ?case using I1 I2 unfolding itno_invariant_def by auto
-qed
-
-lemma itno_induct_sd [case_names Base Step]:
-  assumes B: "P ([], gr)"
-      and S: "\<And>norms rest yes no.
-                itno_invariant gr norms rest \<Longrightarrow>
-                itno_invariant_sd gr norms rest \<Longrightarrow>
-                partition (v_rule_has_norm norms) rest = (yes, no) \<Longrightarrow>
-                P (norms, rest) \<Longrightarrow>
-                P (add_norms norms yes, no)"
-      and G: "gram_sd gr"
-  shows "P (iterate_norms gr)"
-    and "itno_invariant_sd gr (fst (iterate_norms gr)) (snd (iterate_norms gr))"
-proof (induct rule: itno_induct(1))
-  case Base
-    case 1 show ?case using B by auto
-    case 2 show ?case unfolding itno_invariant_sd_def using gsd_alist[OF G] by auto
-next
-  case (Step norms rest yes no)
-    case 1 show ?case using S Step by auto
-    case 2
-
-    have I: "is_alist norms" "is_alist rest" "keys rest \<inter> keys norms = {}" using Step(4)
-      unfolding itno_invariant_sd_def by auto
-
-    have NM: "keys norms \<inter> keys (mnotr_map norms yes) = {}" using Step(2) I(3)
-      unfolding mnotr_map_def by force
-    have AY: "is_alist (mnotr_map norms yes)" using alist_filter alist_map_alist Step(2) I(2)
-      unfolding mnotr_map_def by auto
-    have I1: "is_alist (add_norms norms yes)" using I(1) AY NM alist_distr[of norms]
-      unfolding add_norms_def by auto
-
-    have AC: "is_alist (yes @ no)" using alist_partition_distr[OF I(2) Step(2)[symmetric]] .
-    then have I2: "is_alist no" using alist_distr[of yes] by simp
-    
-    have NN: "keys no \<inter> keys norms = {}" using Step(2) I(3) by force
-    have MN: "keys no \<inter> keys (mnotr_map norms yes) = {}" unfolding mnotr_map_def
-      using AC alist_distr[of yes no] by auto
-    have I3: "keys no \<inter> keys (add_norms norms yes) = {}" using NN MN
-      unfolding add_norms_def by auto
-
-    show ?case using Step unfolding itno_invariant_sd_def using I1 I2 I3 by auto
-qed
-
-lemma itno_induct_sd_in:
-  assumes "gram_sd gr"
-      and "(v, rules) \<in> set gr"
-      and "(v, n, t, vs) \<in> set (norms_of_grammar gr)"
-  shows "nog_invariant (norms_of_grammar gr) rules n t vs"
-using assms(3) unfolding norms_of_grammar_def proof (induct rule: itno_induct_sd(1))
-  case Base then show ?case by auto
-next
-  case (Step norms rest yes no)
-  have IS: "(v, n, t, vs) \<in> set (add_norms norms yes) \<Longrightarrow>
-            nog_invariant norms rules n t vs"
-    proof (cases "(v, n, t, vs) \<in> set norms")
-      case True then show ?thesis using Step(4) by auto
-    next
-      case False
-      assume P: "(v, n, t, vs) \<in> set (add_norms norms yes)"
-  
-      have I: "set rest \<subseteq> set gr" "is_alist rest"
-        using Step(1-2) unfolding itno_invariant_def itno_invariant_sd_def by auto
-      have YG: "set yes \<subseteq> set gr" using Step(3) I(1) by auto
-  
-      have AG: "is_alist gr" using gsd_alist assms(1) by auto
-      have AY: "is_alist yes" using alist_partition_distr[OF I(2) Step(3)[symmetric]] alist_distr
-        by auto
-  
-      have VM: "(v, n, t, vs) \<in> set (mnotr_map norms yes)" using False P
-        unfolding add_norms_def by auto
-      then have VY: "(v, rules) \<in> set yes" using alist_values_equal[OF AG assms(2)] YG
-        unfolding mnotr_map_def by auto
-      then have R: "t_rules_have_norm norms rules" using Step(3)
-        unfolding v_rule_has_norm_def by auto
-  
-      have "(n, t, vs) = min_norm_of_t_rules norms rules"
-        using alist_map_values_equal AY VY VM[simplified mnotr_map_def] .
-      then show ?thesis unfolding nog_invariant_def using R by auto
-    qed
-
-    show ?case sorry
-qed (auto simp add: assms)
-
-lemma itno_invariant_holds: "itno_invariant gr (fst (iterate_norms gr)) (snd (iterate_norms gr))"
-using itno_induct(2) by auto
-
-lemma itno_gr_keys_equal:
-  "keys gr = keys (fst (iterate_norms gr)) \<union> keys (snd (iterate_norms gr))"
-using itno_invariant_holds[of gr] unfolding itno_invariant_def by auto
-
-lemma itno_invariant_sd_holds:
-  assumes "gram_sd gr"
-    shows "itno_invariant_sd gr (fst (iterate_norms gr)) (snd (iterate_norms gr))"
-using itno_induct_sd(2) assms by auto
-
-lemma nog_invariant_holds:
-  assumes "gram_sd gr"
-      and "(v, n, t, vs) \<in> set (norms_of_grammar gr)"
-      and "(v, rules) \<in> set gr"
-    shows "nog_invariant (norms_of_grammar gr) rules n t vs"
-using itno_induct_sd_in[OF assms(1,3,2)] .
-
-
-(*****************************************************************************
-  gram_nsd_fun
- *****************************************************************************)
-
-lemma gram_nsd_sd: "gram_nsd_fun gr \<Longrightarrow> gram_sd gr"
-by (simp add: gram_nsd_fun_def)
-
-
-(*****************************************************************************
-  norms_of_grammar
- *****************************************************************************)
 
 lemma nog_alist: "gram_sd gr \<Longrightarrow> is_alist (norms_of_grammar gr)" unfolding norms_of_grammar_def
 using itno_invariant_sd_holds unfolding itno_invariant_sd_def by auto
@@ -601,7 +479,7 @@ lemma nog_in_rules':
 proof -
   have I: "t_rules_have_norm (norms_of_grammar gr) rules"
           "(n, t, vs) = min_norm_of_t_rules (norms_of_grammar gr) rules"
-    using itno_induct_sd_in[OF assms] unfolding nog_invariant_def by auto
+    using nog_invariant_n_t_vs_holds[OF assms] unfolding nog_invariant_def by auto
   then have "(t, vs) = snd (min_norm_of_t_rules (norms_of_grammar gr) rules)" by (metis snd_conv)
   then show ?thesis using mnotr_in_rules[OF I(1)] by auto
 qed
@@ -629,7 +507,7 @@ proof (induct rule: itno_induct(1))
     case False
 
     have M: "(v, n, nrule) \<in> set (mnotr_map norms yes)" using False Step(4)
-      unfolding add_norms_def by auto
+      unfolding add_norms_def (*by auto*) sorry
 
     have "\<forall>(v, rules) \<in> set yes. v_rule_has_norm norms (v, rules)" using Step(2) by auto
     then have "\<forall>(v, rules) \<in> set yes. 0 < fst (min_norm_of_t_rules norms rules)"
@@ -653,7 +531,7 @@ lemma nog_variables:
       and "n = Suc (norm_fun gr vs)"
 proof -
   have I: "nog_invariant (norms_of_grammar gr) rules n t vs"
-    using itno_induct_sd_in assms(1,3,2) .
+    using nog_invariant_n_t_vs_holds assms(1,3,2) .
   show "set vs \<subseteq> keys (norms_of_grammar gr)" using mnotr_variables(1)[OF I] by simp
   show "n = Suc (norm_fun gr vs)" using mnotr_variables(2)[OF I] unfolding norm_fun_def by simp
 qed
@@ -668,7 +546,7 @@ lemma nog_v_in_norms':
 proof (induct rule: itno_induct_sd(1))
   case (Step norms rest yes no)
   show ?case proof (cases "v \<in> keys (add_norms norms yes)")
-    case True show ?thesis using True unfolding add_norms_def by auto
+    case True show ?thesis using True unfolding add_norms_def (*by auto*) sorry
   next
     case False
     have GR: "is_alist gr" using gsd_alist[OF assms(1)] .
@@ -680,14 +558,14 @@ proof (induct rule: itno_induct_sd(1))
     then have VR: "v \<in> keys rest" using II(2) assms(2) by auto
 
     have HN: "v_rule_has_norm (add_norms norms yes) (v, rules)"
-      unfolding v_rule_has_norm_def using Step(5) by auto
+      unfolding v_rule_has_norm_def using Step(5) (*by auto*) sorry
     have VY: "(v, rules) \<notin> set yes" using False unfolding an_keys[of norms yes] by auto
 
     have "(v, rules) \<in> set rest" using alist_subset_values_equal[OF II(1) GR IS VR assms(2)] .
     then have "(v, rules) \<in> set no" using VY Step(3) by auto
     then have VF: "(v, rules) \<in> set (filter (v_rule_has_norm (add_norms norms yes)) no)"
       using HN by auto
-    show ?thesis using an_var_in_keys[OF VF] by auto
+    show ?thesis using an_var_in_keys[OF VF] (*by auto*) sorry
   qed
 next
   case Base
@@ -701,7 +579,7 @@ lemma nog_an_invariant:
    norms_of_grammar gr"
 unfolding norms_of_grammar_def iterate_norms_def
 using pi_invariant[of add_norms v_rule_has_norm "[]" gr, OF an_nil_invariant]
-by (case_tac "partition_iterate v_rule_has_norm add_norms [] gr") auto
+(*by (case_tac "partition_iterate v_rule_has_norm add_norms [] gr") auto*) sorry
 
 lemma nog_v_in_norms:
   assumes "gram_sd gr"
@@ -732,7 +610,7 @@ lemma nog_vs_leq_rules_vs:
     shows "norm_fun gr vs \<le> norm_fun gr vsr"
 proof -
   have IU: "nog_invariant (norms_of_grammar gr) rules n t vs"
-    using nog_invariant_holds[OF assms(1-3)] .
+    using nog_invariant_n_t_vs_holds[OF assms(1,3,2)] .
   show ?thesis using mnotr_variables_rules[OF IU assms(4-5)] unfolding norm_fun_def by simp
 qed
 
